[OK] check (now it compiles with some admit)

theories/check.v
@@ -8,7 +8,7 @@ From HB Require Import structures.
 Require Import FunInd.
 Functional Scheme expand_ind := Induction for step Sort Prop.
 
-Definition sV_expand (S:sigV) Sexp:=
+(* Definition sV_expand (S:sigV) Sexp:=
   forall k, 
     match lookup k Sexp with
     | None => True
@@ -22,18 +22,17 @@ Proof.
   move=> //k.
   case lookup => //= s.
   rewrite incl_refl//.
-Qed.
+Qed. *)
 
 Lemma expand_det_tree {u sP sV sV' A r s ign d} : 
   check_program sP ->
-    sigma2ctx sP s = Some sV ->
-      tc_tree_aux sP sV A ign = ty_ok (d, sV') ->
+    sigma2ctx sP s = sV ->
+      tc_tree_aux sP sV A ign = (d, sV') ->
         step u s A = r ->
           exists S d', minD d d' = d' /\ 
           (* sV_expand sV' S /\ *)
-            tc_tree_aux sP sV (get_tree r) d = ty_ok (d', S).
+            tc_tree_aux sP sV (get_tree r) d = (d', S).
 Proof.
-  simpl in *.
   move=> C.
   move: sV sV' r d ign.
   pattern u, s, A, (step u s A).
@@ -50,7 +49,6 @@ Proof.
       -  admit.
     }
   - move=> s []//= _ ???? _ _ [_ ->] <-/=; repeat eexists; rewrite ?minD_refl//.
-    (* apply: sV_expand_refl. *)
   - move=> s INIT A sB B HINIT dA IH sV sV' r d ign H/=.
     rewrite is_dead_is_ko//=.
     have ?: sB = s by admit.
@@ -59,26 +57,30 @@ Proof.
     rewrite get_tree_Or /= is_dead_is_ko//.
     apply: IH; eauto.
   - move=> s INIT A sB B HINIT dA IH A' eA sV sV' r d ign H/=.
-    case: ifP => kA.
-      by rewrite is_ko_step in eA.
+    case: ifP => kA; first by rewrite is_ko_step in eA.
+    case: ifP => kB.
+      move=> dtA <-{r}/=.
+      rewrite kB.
+      have {IH}/=[S[d'[H1 H2]]]:= IH _ _ _ _ _ H dtA eA.
+      rewrite H2.
+      have:= is_ko_tc_tree_aux kB.
+      move=> /(_ sP sV d) ->; case: ifP; repeat eexists; eauto.
+      rewrite minD_refl//.
     have fA:= expand_not_failed _ eA notF.
     move=> + <-{r}/=.
-    (* case nB: next_alt => [B'|]//=. *)
-    case dtA: (tc_tree_aux _ _ A) => /=[[DA' sVA]|]//=.
-    case dtB: (tc_tree_aux _ _ B) => /=[[DB sVB]|]//=.
-    case M: merge_sig => //=[S']; subst.
+    case dtA: (tc_tree_aux _ _ A) => /=[DA' sVA]//=.
+    case dtB: (tc_tree_aux _ _ B) => /=[DB sVB]//=.
     have {IH}/=[S[d'[H1 H2]]]:= IH _ _ _ _ _ H dtA eA.
     move=> [??]; subst.
     case kA' : (is_ko A'); last first.
       rewrite (expand_Exp_has_cut eA).
-      have:= same_ty_tc_tree_aux sP sV A' DA' (if has_cut A' then maxD DA' DB else Pred).
+      have:= same_ty_tc_tree_aux sP (sigma2ctx sP s) A' DA' (if has_cut A' then maxD DA' DB else Pred).
       rewrite H2/=.
-      case dtA2: (tc_tree_aux _ _ A') => /=[[DA2 sVA2]|]//=/eqP[?]; subst sVA2.
-      have:= same_ty_tc_tree_aux sP sV B ign (if has_cut A' then maxD DA' DB else Pred).
+      case dtA2: (tc_tree_aux _ _ A') => /=[DA2 sVA2]//=?; subst sVA2.
+      have:= same_ty_tc_tree_aux sP (sigma2ctx sP s) B ign (if has_cut A' then maxD DA' DB else Pred).
       rewrite dtB.
-      case dtB1: (tc_tree_aux _ _ B) => /=[[DB2 sVB2]|]//=/eqP[?]; subst sVB2.
-      have: exists T, merge_sig S sVB = ty_ok T by admit.
-      move=> [SS HH]; rewrite HH/=.
+      case dtB1: (tc_tree_aux _ _ B) => /=[DB2 sVB2] ?; subst sVB2.
+      rewrite kB.
       move: dtA2 dtB1.
       case: ifP; repeat eexists => //=.
       destruct DA', DB => //=; simpl in *; subst.
@@ -88,108 +90,110 @@ Proof.
       by destruct d2.
     rewrite (expand_Exp_has_cut eA) failed_has_cut?is_ko_failed//.
     move=> /=.
-    have:= same_ty_tc_tree_aux sP sV B ign Pred.
-    rewrite dtB; case dtB': tc_tree_aux => //=[[D1 S1]]; repeat eexists.
+    have:= same_ty_tc_tree_aux sP (sigma2ctx sP s) B ign Pred.
+    rewrite dtB; case dtB': tc_tree_aux => //=[D1 S1]; repeat eexists.
   - move=> s INIT A sB B HINIT dA IH A' eA sV sV' r d ign H/=.
-    case: ifP => kA.
-      by rewrite is_ko_step in eA.
+    case: ifP => kA; first by rewrite is_ko_step in eA.
+    case: ifP => kB.
+      move=> dtA <-/=.
+      rewrite (expand_CB_is_ko eA) is_ko_cutr.
+      by apply: IH H dtA eA.
     have fA:= expand_not_failed _ eA notF.
-    case dtA: (tc_tree_aux _ _ A) => /=[[DA' sVA]|]//=.
-    case dtB: (tc_tree_aux _ _ B) => /=[[DB sVB]|]//=.
-    case M: merge_sig => //=[S']; subst.
-    move=> [??]; subst.
-    have {IH}/=[S[d' [H1 H2]]] := IH _ _ _ _ _ H dtA eA.
-    have := same_ty_tc_tree_aux sP sV A' DA' (if has_cut A then maxD DA' DB else Pred).
-    rewrite H2/= => /eqP.
-    case Hz : tc_tree_aux => //=[[Dx sX]][?]; subst sX.
-    move=> <-{r}/=.
-    rewrite Hz/=.
-    rewrite (expand_CB_is_ko eA).
-    have V := sigma2ctx_valid H.
-    have:= @cutr_tc_tree_aux sP sV B (if has_cut A then maxD DA' DB else Pred) V.
-    move=> [SB dtB']; rewrite dtB'/=.
-    have: exists T, merge_sig S sV = ty_ok T by admit.
-    move=> [SS HH]; rewrite HH/=.
-    move: Hz dtB'.
-    case: ifP => cA Hz dtB'; repeat eexists.
-    case cA': (has_cut A').
-      destruct DA', DB => //=; simpl in *; subst.
-      destruct Dx; [|congruence] => /=.
-      (* TODO: this is not provable in the current setting, should change the definition of tc_tree_aux if cutr is rhs of OR? *)
-      admit.
-    destruct DA'; simpl in *; subst => //.
-    destruct DB => //=.
-    admit.
+    case dtA: (tc_tree_aux _ _ A) => /=[DA' sVA]//=.
+    case dtB: (tc_tree_aux _ _ B) => /=[DB sVB]//=.
+    move=> [??]<-; subst => /=.
+    rewrite (expand_CB_is_ko eA) is_ko_cutr.
+    have {IH}/=[S[d' [H1 /=H2]]] := IH _ _ _ _ _ erefl dtA eA.
+    have := same_ty_tc_tree_aux sP (sigma2ctx sP s) A' DA' (if has_cut A then maxD DA' DB else Pred).
+    rewrite H2/=.
+    case Hz : tc_tree_aux => //=[Dx sX] ?; subst sX.
+    move: Hz; case: ifP => cA Hz/=; repeat eexists.
+    destruct DA', DB, d', Dx; simpl in *; congruence.
   - move=> s INIT A sB B HINIT dA IH A' eA sV sV' r d ign H/=.
     have [? fA] := expand_failed_same _ eA; subst A'.
     case: ifP => kA.
       move=> dtB <-/=; rewrite kA.
       have:= same_ty_tc_tree_aux sP sV B ign d.
       rewrite dtB.
-      case dtB': tc_tree_aux => //=[[D1 S1]]/=/eqP[?]; subst.
+      case dtB': tc_tree_aux => //=[D1 S1]/=?; subst.
       repeat eexists; destruct d => //=.
       have:= tc_tree_aux_func2 dtB; rewrite dtB'.
-      move=> [][]//=[]// _ []//.
+      by move=> [][]//=[]// _ []//.
+    case: ifP => kB.
+      move=> dtA <-{r}/=; rewrite kB kA.
+      have:= same_ty_tc_tree_aux sP sV A ign d.
+      rewrite dtA.
+      case dtB': tc_tree_aux => //=[D1 S1]/=/eqP?; subst.
+      repeat eexists; destruct d => //=.
+      have:= tc_tree_aux_func2 dtA; rewrite dtB'.
+      by move=> [][]//=[]// _ []//.
     move=> +<-{r}/=.
     have:= same_ty_tc_tree_aux sP sV A ign d.
-    case dtA1: (tc_tree_aux _ _ A) => /=[[DA1 sVA1]|]//=.
-    case dtA2: (tc_tree_aux _ _ A) => /=[[DA2 sVA2]|]//=/eqP[?]; subst sVA2.
+    case dtA1: (tc_tree_aux _ _ A) => /=[DA1 sVA1]//=.
+    case dtA2: (tc_tree_aux _ _ A) => /=[DA2 sVA2]//=?; subst sVA2.
     have:= same_ty_tc_tree_aux sP sV B ign d.
-    case dtB1: (tc_tree_aux _ _ B) => /=[[DB1 sVB1]|]//=.
-    case dtB2: (tc_tree_aux _ _ B) => /=[[DB2 sVB2]|]//=/eqP[?]; subst sVB2.
-    case M: merge_sig => //=[S'][??]; subst.
-    rewrite kA.
-    repeat eexists; case:ifP => //=.
-    rewrite failed_has_cut//=.
+    case dtB1: (tc_tree_aux _ _ B) => /=[DB1 sVB1]//=.
+    case dtB2: (tc_tree_aux _ _ B) => /=[DB2 sVB2]//=?; subst sVB2.
+    rewrite kA kB.
+    rewrite failed_has_cut//= => -[??]; subst.
+    repeat eexists.
   - move=> s INIT A sB B HINIT dA IH A' eA sV sV' r d ign H/=.
     have [? sA]:= expand_solved_same _ eA; subst A'.
     rewrite success_is_ko//=.
     move=> +<-{r}/=.
     rewrite success_has_cut//=.
     have:= same_ty_tc_tree_aux sP sV A ign d.
-    case dtA1: (tc_tree_aux _ _ A) => /=[[DA1 sVA1]|]//=.
-    case dtA2: (tc_tree_aux _ _ A) => /=[[DA2 sVA2]|]//=/eqP[?]; subst sVA2.
+    case dtA1: (tc_tree_aux _ _ A) => /=[DA1 sVA1]//=.
+    case dtA2: (tc_tree_aux _ _ A) => /=[DA2 sVA2]//=?; subst sVA2.
     have:= same_ty_tc_tree_aux sP sV B ign d.
-    case dtB1: (tc_tree_aux _ _ B) => /=[[DB1 sVB1]|]//=.
-    case dtB2: (tc_tree_aux _ _ B) => /=[[DB2 sVB2]|]//=/eqP[?]; subst sVB2.
-    case M: merge_sig => //=[S'][??]; subst.
-    rewrite success_is_ko//.
-    repeat eexists.
-  - move=> s INIT A B0 B HINIT IH A' eA sV sV' r d ign H/= + <-/=.
+    case dtB1: (tc_tree_aux _ _ B) => /=[DB1 sVB1]//=.
+    case dtB2: (tc_tree_aux _ _ B) => /=[DB2 sVB2]//=?; subst sVB2.
+    case: ifP => kB [??]; subst; rewrite success_is_ko//; repeat eexists.
+    destruct d, DA2 => //=.
+    have:= tc_tree_aux_func2 dtA1.
+    rewrite dtA2 => -[[] []] <-//.
+  - move=> s INIT A B0 B HINIT IH A' eA sV r d ign H/= <-/= + <-.
     have fA:= expand_not_failed _ eA notF.
     have sA:= expand_not_solved_not_success _ eA notF.
-    case dtA1: (tc_tree_aux _ _ A) => /=[[DA1 sVA1]|]//=.
-    case dtB01: (tc_tree_aux _ _ B0) => /=[[DB01 sVB01]|]//=.
-    case dtB1: (tc_tree_aux _ _ B) => /=[[DB1 sVB1]|]//=.
-    case M: merge_sig => //=[S'][??]; subst.
-    have {IH}/=[S[d'[H1 H2]]] := IH _ _ _ _ _ H dtA1 eA.
-    have:= same_ty_tc_tree_aux sP sV A' DA1 (maxD DB01 DB1).
+    rewrite failed_is_ko//=.
+    case dtA1: (tc_tree_aux _ _ A) => /=[DA1 sVA1]//=.
+    case dtB01: (tc_tree_aux _ _ B0) => /=[DB01 sVB01]//=.
+    case dtB1: (tc_tree_aux _ _ B) => /=[DB1 sVB1]//=[??]; subst.
+    (* case M: merge_sig => //=[S'][??]; subst. *)
+    have {IH}/=[S[d'[H1 H2]]] := IH _ _ _ _ _ erefl dtA1 eA.
+    have:= same_ty_tc_tree_aux sP ((sigma2ctx sP s)) A' DA1 (maxD DB01 DB1).
     rewrite H2.
-    case dtA1': (tc_tree_aux _ _ A') => /=[[DA1' sVA1']|]//=/eqP[?]; subst sVA1'.
+    case dtA1': (tc_tree_aux _ _ A') => /=[DA1' sVA1']//=?; subst sVA1'.
+    case: ifP => kA; first by repeat eexists; rewrite minD_refl.
     admit. (*TODO: pb with tc_tree_aux ran with a more precise subst then the hyp, should be solved using more_precise_tc_tree_aux *)
-  - move=> s INIT A B0 B HINIT IH A' eA sV sV' r d ign H/=.
-    case dtA: (tc_tree_aux _ _ A) => /=[[DA' sVA]|]//=.
-    case dtB0: (tc_tree_aux _ _ B0) => /=[[DB0 sVB0]|]//=.
-    case dtB: (tc_tree_aux _ _ B) => /=[[DB sVB]|]//=.
-    case M: merge_sig => //=[S'][??]; subst.
-    move=> <-{r}/=.
+  - move=> s INIT A B0 B HINIT IH A' eA sV r d ign H/= <- +<-.
+    have fA:= expand_not_failed _ eA notF.
+    rewrite failed_is_ko//=.
+    case dtA: (tc_tree_aux _ _ A) => /=[DA' sVA]//=.
+    case dtB0: (tc_tree_aux _ _ B0) => /=[DB0 sVB0]//=.
+    case dtB: (tc_tree_aux _ _ B) => /=[DB sVB]//=[??]; subst.
+    case:ifP => kA; first by repeat eexists; rewrite minD_refl.
+    have {IH}/=[S[d'[H1 H2]]] := IH _ _ _ _ _ erefl dtA eA.
+    have:= same_ty_tc_tree_aux sP ((sigma2ctx sP s)) A' DA' (maxD DB0 DB).
+    rewrite H2.
+    case dtA1': (tc_tree_aux _ _ A') => /=[DA1' sVA1']//=?; subst sVA1'.
     admit. (*same as above...*)
-  - move=> s INIT A B0 B HINIT IH A' eA sV sV' r d ign H/=.
-    have [? fA]:= expand_failed_same _ eA; subst A' => +<-{r}/=.
-    case dtA: (tc_tree_aux _ _ A) => /=[[DA' sVA]|]//=.
-    case dtB0: (tc_tree_aux _ _ B0) => /=[[DB0 sVB0]|]//=.
-    case dtB: (tc_tree_aux _ _ B) => /=[[DB sVB]|]//=.
-    case M: merge_sig => //=[S'][??]; subst.
-    have:= same_ty_tc_tree_aux sP sV A ign (maxD DB0 DB).
+  - move=> s INIT A B0 B HINIT IH A' eA sV sV' r d ign/= <- +<-/=.
+    have [? fA]:= expand_failed_same _ eA; subst A'.
+    case:ifP => kA; first by move=> [??]; subst; repeat eexists; rewrite minD_refl.
+    case dtA: (tc_tree_aux _ _ A) => /=[DA' sVA]//=.
+    case dtB0: (tc_tree_aux _ _ B0) => /=[DB0 sVB0]//=.
+    case dtB: (tc_tree_aux _ _ B) => /=[DB sVB]//=[??]; subst.
+    have:= same_ty_tc_tree_aux sP (sigma2ctx sP s) A ign (maxD DB0 DB).
     rewrite dtA.
-    case dtA1: (tc_tree_aux _ _ A) => /=[[DA1 sVA1]|]//=/eqP[?]; subst sVA1.
+    case dtA1: (tc_tree_aux _ _ A) => /=[DA1 sVA1]//=?; subst sVA1.
     have:= same_ty_tc_tree_aux sP sVA B DA' DA1.
     rewrite dtB/=.
-    case dtB1: (tc_tree_aux _ _ B) => /=[[DB1 sVB1]|]//=/eqP[?]; subst sVB1.
+    case dtB1: (tc_tree_aux _ _ B) => /=[DB1 sVB1]//=?; subst sVB1.
     have:= same_ty_tc_tree_aux sP sVA B0 DA' DA1.
     rewrite dtB0/=.
-    case dtB01: (tc_tree_aux _ _ B0) => /=[[DB01 sVB01]|]//=/eqP[?]; subst sVB01.
-    rewrite M/=; repeat eexists.
+    case dtB01: (tc_tree_aux _ _ B0) => /=[DB01 sVB01]//=?; subst sVB01.
+    repeat eexists.
     destruct DB0,DB => //=; simpl in *.
     destruct DA'; simpl in *; last first.
       have [[][// _ H1]] := tc_tree_aux_func2 dtB0.
@@ -200,35 +204,63 @@ Proof.
       move: dtB01; rewrite dtB0 => -[<-]/=; congruence.
     have [[][//= _]] := tc_tree_aux_func2 dtA.
     rewrite dtA1 => -[?]; subst.
-    destruct DB01;[|congruence] => /=; congruence.
-  - move=> s INIT A B0 B HINIT HL A' eA HR sV sV' r d ign H/= + <-{r}/=.
-    case dtA: (tc_tree_aux _ _ A) => /=[[DA' sVA]|]//=.
-    case dtB0: (tc_tree_aux _ _ B0) => /=[[DB0 sVB0]|]//=.
-    case dtB: (tc_tree_aux _ _ B) => /=[[DB sVB]|]//=.
-    case M: merge_sig => //=[S'][??]; subst.
+    destruct DB01 => /=;congruence.
+  - move=> s INIT A B0 B HINIT HL A' eA HR sV sV' r d ign <-/= +<-/=.
     have [? sA] := expand_solved_same _ eA; subst A'.
-    case eB: step => //=[B'|B'|B'|B'].
-    - have:= same_ty_tc_tree_aux sP sV A ign (maxD DB0 DB).
+    rewrite success_is_ko//=.
+    case dtA: (tc_tree_aux _ _ A) => /=[DA' sVA]//=.
+    case dtB0: (tc_tree_aux _ _ B0) => /=[DB0 sVB0]//=.
+    case dtB: (tc_tree_aux _ _ B) => /=[DB sVB]//=.
+    move=> [??]; subst.
+    case eB: step => //=[B'|B'|B'|B']; rewrite success_is_ko//?success_cut//.
+    - have:= same_ty_tc_tree_aux sP (sigma2ctx sP s) A ign (maxD DB0 DB).
       rewrite dtA.
-      case dtA1: (tc_tree_aux _ _ A) => /=[[DA1 sVA1]|]//=/eqP[?]; subst sVA1.
+      case dtA1: (tc_tree_aux _ _ A) => /=[DA1 sVA1]//=?; subst sVA1.
       have:= same_ty_tc_tree_aux sP sVA B0 DA' DA1.
       rewrite dtB0/=.
-      case dtB01: (tc_tree_aux _ _ B0) => /=[[DB01 sVB01]|]//=/eqP[?]; subst sVB01.
-      have:= HR _ _ _ _ _ _ dtB eB.
+      case dtB01: (tc_tree_aux _ _ B0) => /=[DB01 sVB01]//=?; subst sVB01.
+      (* have: exists XX, sigma2ctx sP (get_substS s A) = Some XX /\ more_precise XX sVA.
+        admit.
+      move=> [XX [HH ZZ]].
+      have:= HR _ _ _ _ _ _ HH ZZ dtB eB.
+      move=> /=[S1[D1[Hx Hy]]].
+      have:= same_ty_tc_tree_aux sP sVA B' DB DA1.
+      rewrite Hy.
+      case dtB': tc_tree_aux => //=[[D S]]/eqP[?]; subst S.
+      have: exists T, merge_sig S1 sVB0 = ty_ok T by admit.
+      move=> [T H1]; rewrite H1; repeat eexists.
+      destruct DB0, DB; simpl in *; subst => //=.
+      have:= tc_tree_aux_func2 dtA.
+      rewrite dtA1/= => -[d2[H2 [?]]]; subst.
+      have:= tc_tree_aux_func2 dtB'.
+      rewrite Hy/= => -[d3[H3 [?]]]/=; subst.
+      simpl in *; subst.
+      have [d3[H4 H5]] := tc_tree_aux_func2 dtB01.
+      destruct d2; simpl in *; subst.
+        destruct D; try congruence.
+        destruct DB01, d3; try congruence.
+
+      destruct d3; simpl in *; subst => //=.
+      rewrite dtB0/= => -[d4[H4 [?]]]/=; subst.
+      simpl in *; subst.
+      destruct DB01 => //=.
+
+      rewrite Hy. *)
       admit. (*PB with ctx*)
-    - (*TODO: pb with cutl: no lemma for it...*)
-       admit.
+    - rewrite cutl_tc_tree_aux// cutr_tc_tree_aux.
+      have /= := HR _ _ _ _ _ _ dtB eB.
+      admit. (*PB with ctx*)
     - have [? fB] := expand_failed_same _ eB; subst B'.
-      have:= same_ty_tc_tree_aux sP sV A ign (maxD DB0 DB).
+      have:= same_ty_tc_tree_aux sP (sigma2ctx sP s) A ign (maxD DB0 DB).
       rewrite dtA.
-      case dtA1: (tc_tree_aux _ _ A) => /=[[DA1 sVA1]|]//=/eqP[?]; subst sVA1.
+      case dtA1: (tc_tree_aux _ _ A) => /=[DA1 sVA1]//=?; subst sVA1.
       have:= same_ty_tc_tree_aux sP sVA B0 DA' DA1.
       rewrite dtB0/=.
-      case dtB01: (tc_tree_aux _ _ B0) => /=[[DB01 sVB01]|]//=/eqP[?]; subst sVB01.
+      case dtB01: (tc_tree_aux _ _ B0) => /=[DB01 sVB01]//=?; subst sVB01.
       have:= same_ty_tc_tree_aux sP sVA B DA' DA1.
       rewrite dtB/=.
-      case dtB1: (tc_tree_aux _ _ B) => /=[[DB1 sVB1]|]//=/eqP[?]; subst sVB1.
-      rewrite M/=; repeat eexists.
+      case dtB1: (tc_tree_aux _ _ B) => /=[DB1 sVB1]//=?; subst sVB1.
+      repeat eexists.
       destruct DB0, DB => //=; simpl in *.
       destruct DA'; simpl in *; last first.
         have [[][// _ H1]] := tc_tree_aux_func2 dtB0.
@@ -239,18 +271,18 @@ Proof.
         move: dtB01; rewrite dtB0 => -[<-]/=; congruence.
       have [[][//= _]] := tc_tree_aux_func2 dtA.
       rewrite dtA1 => -[?]; subst.
-      destruct DB01;[|congruence] => /=; congruence.
+      destruct DB01 => /=; congruence.
     - have [? sB]:= expand_solved_same _ eB; subst B'.
-      have:= same_ty_tc_tree_aux sP sV A ign (maxD DB0 DB).
+      have:= same_ty_tc_tree_aux sP (sigma2ctx sP s) A ign (maxD DB0 DB).
       rewrite dtA.
-      case dtA1: (tc_tree_aux _ _ A) => /=[[DA1 sVA1]|]//=/eqP[?]; subst sVA1.
+      case dtA1: (tc_tree_aux _ _ A) => /=[DA1 sVA1]//=?; subst sVA1.
       have:= same_ty_tc_tree_aux sP sVA B0 DA' DA1.
       rewrite dtB0/=.
-      case dtB01: (tc_tree_aux _ _ B0) => /=[[DB01 sVB01]|]//=/eqP[?]; subst sVB01.
+      case dtB01: (tc_tree_aux _ _ B0) => /=[DB01 sVB01]//=?; subst sVB01.
       have:= same_ty_tc_tree_aux sP sVA B DA' DA1.
       rewrite dtB/=.
-      case dtB1: (tc_tree_aux _ _ B) => /=[[DB1 sVB1]|]//=/eqP[?]; subst sVB1.
-      rewrite M/=; repeat eexists.
+      case dtB1: (tc_tree_aux _ _ B) => /=[DB1 sVB1]//=?; subst sVB1.
+      repeat eexists.
       destruct DB0, DB => //=; simpl in *.
       destruct DA'; simpl in *; last first.
         have [[][// _ H1]] := tc_tree_aux_func2 dtB0.
@@ -261,7 +293,7 @@ Proof.
         move: dtB01; rewrite dtB0 => -[<-]/=; congruence.
       have [[][//= _]] := tc_tree_aux_func2 dtA.
       rewrite dtA1 => -[?]; subst.
-      destruct DB01;[|congruence] => /=; congruence.
+      destruct DB01 => /=; congruence.
 Admitted.
 
 Definition is_det s A := forall u s' B n,
@@ -269,8 +301,8 @@ Definition is_det s A := forall u s' B n,
 
 Lemma run_is_det {sP sV sV' s A}: 
   check_program sP -> 
-    sigma2ctx sP s = Some sV ->
-    tc_tree_aux sP sV A Func = ty_ok (Func, sV') -> is_det s A.
+    sigma2ctx sP s = sV ->
+    tc_tree_aux sP sV A Func = (Func, sV') -> is_det s A.
 Proof.
   rewrite/is_det.
   move=> ckP ++ u s' B n H.
@@ -279,18 +311,18 @@ Proof.
     by have /=-> := success_det_tree_next_alt sA H2.
   - move=> s1 s2 r A B n eA _ IH sV sV' H1 dtA.
     have /= [S' [d [<- H]]]:= expand_det_tree ckP H1 dtA eA; subst.
-    apply: IH (H1) H.
+    by apply: IH H.
   - move=> s1 s2 r A B n eA _ IH sV sV' H1 dtA.
     have /= [S' [d [<- H]]]:= expand_det_tree ckP H1 dtA eA; subst.
-    apply: IH (H1) H.
+    by apply: IH H.
   - move=> s1 s2 A B r n fA nA _ IH sV sV' H1 H2.
-    have V := sigma2ctx_valid H1.
-    have := failed_det_tree_next_alt false V H2 nA.
+    have cA: closed_inT sV A by admit.
+    have := failed_det_tree_next_alt cA H2 nA.
     move => -[[]// [s [? [X _]]]]//.
-    apply: IH (H1) X.
+    by apply: IH X.
   - move=> *.
     rewrite is_dead_next_alt//is_dead_dead//.
-Qed.
+Admitted.
 
 Definition det_tree sP A := typ_func (tc_tree_aux sP empty_ctx A Func).
 
@@ -299,10 +331,11 @@ Lemma main {sP p t}:
     is_det empty ((CallS p t)).
 Proof.
   rewrite /det_tree/is_det.
-  case D: tc_tree_aux => //=[[[] S]]//=.
-  move=> H1 H2 u s' B n H.
+  move=> /=.
+  case C: check_callable => [[] S]//= CP _.
+  move=> u s' B n H.
   apply: run_is_det H; eauto.
-  rewrite/sigma2ctx//.
+  rewrite sigma2ctx_empty/= C//.
 Qed.
 
 Print Assumptions  main.
@@ -312,11 +345,11 @@ Module elpi.
   From det Require Import tree t2l_prop tree_valid_state tree_prop.
 
   Definition is_det g := forall u s' a',
-    nur u [::] g nilC s' a' -> a' = nilC.
+    nur u empty g nilC s' a' -> a' = nilC.
 
   Lemma elpi_is_det {sP p c ign}: 
     check_program sP -> 
-      check_callable sP [::] c Func = ty_ok (Func, ign) -> 
+      check_callable sP empty_ctx c Func = (Func, ign) -> 
       is_det ((call p c):::nilC).
   Proof.
     simpl in *.
@@ -324,7 +357,7 @@ Module elpi.
     move=> /elpi_to_tree /(_ _ (CallS p c))/=.
     move=> /(_ _ isT erefl) [t1'[n [H3 H4]]].
     have /= := run_is_det H1 .
-    move=> /(_ [::] ign [::] (CallS p c) erefl)/=.
+    move=> /(_ empty_ctx ign empty (CallS p c) (sigma2ctx_empty _))/=.
     rewrite H2/= => /(_ erefl).
     (* rewrite H2/= => /(_ isT). *)
     rewrite /check.is_det -H4.
